examples/Dice4_6.ec
@@ -1,13 +1,9 @@
-require import Dice_sampling.
-import Distr.
-import FSet.
-import Int.
-import Real.
+require import Int Real Distr FSet Dice_sampling.
 
 clone GenDice as D4_6 with 
   type t <- int,
   type input <- unit,
-  pred valid = True,
+  pred valid = predT,
   op d (i:unit) <- [1..6],
   op test (i:unit) x <- 1 <= x <= 4,
   op sub_supp (i:unit) <- Interval.interval 1 4,
@@ -33,13 +29,11 @@ module D4 = {
 lemma prD4 : forall k &m, Pr[D4.sample() @ &m : res = k] = 
    if 1 <= k && k <= 4 then 1%r/4%r else 0%r.
 proof.
-  intros k &m; byphoare (_: true ==> k = res) => //.
-  proc;rnd;skip;progress => //.
-  rewrite (_:mu [1..4] (fun (x : int), k = x) = mu_x [1..4] k).
-    by rewrite /mu_x;apply mu_eq.
-  by case (1 <= k && k <= 4) => Hk; 
-    [rewrite Dinter.mu_x_def_in // | rewrite Dinter.mu_x_def_notin //];
-    rewrite Dinter.supp_def. 
+  move=> k &m; byphoare=> //.
+  proc; rnd; skip; progress => //.
+  by rewrite -/(pred1 _) -/(mu_x _ _); case (1 <= k <= 4)=> Hk;
+     [rewrite Dinter.mu_x_def_in|rewrite Dinter.mu_x_def_notin];
+     smt.
 qed.
 
 module D6 = {
@@ -52,12 +46,12 @@ module D6 = {
 }.
 
 equiv D4_Sample : D4.sample ~ D4_6.Sample.sample : true ==> ={res}.
-proof. proc;rnd => //. qed.
+proof. proc; rnd => //. qed.
 
 equiv D6_RsampleW : D6.sample ~ D4_6.RsampleW.sample : r{2} = 5 ==> ={res}.
 proof. 
-  proc;while (={r}).
-    by rnd;skip;progress => //; smt.
+  proc; while (={r}).
+    by rnd; skip; smt.
   by wp.
 qed.
 
@@ -66,26 +60,26 @@ lemma D4_D6 (f finv : int -> int) :
     (forall i, 1 <= i <= 4 => f (finv i) = i /\ finv (f i) = i) =>
     equiv [D4.sample ~ D6.sample : true ==> res{1} = finv res{2}].
 proof.
-  intros Hbound Hbij.
+  move=> Hbound Hbij.
   transitivity D4_6.Sample.sample (true ==> ={res}) (true ==> res{1} = finv res{2}) => //.
     by apply D4_Sample.
   transitivity D4_6.RsampleW.sample (r{2} = 5 ==> res{1} = finv res{2})
       (r{1} = 5 ==> res{2} = res{1}) => //.
-    by intros _ _ _;exists ((),5) => //.
+    by move=> _ _ _;exists ((),5).
     conseq (D4_6.Sample_RsampleW f finv) => //.
-    intros &m1 &m2 -> /=; split; first by smt.
+    move=> &m1 &m2 -> /=; split; first by smt.
     split; first by rewrite /D4_6.valid.
     split; first by rewrite Dinter.weight_def.
-    split; first by intros x;rewrite Dinter.supp_def;apply Hbound.
-    split; first by intros x Hx; cut:= Hbij x _.
-    by intros x; rewrite Dinter.supp_def => Hx; cut:= Hbij x _.
-  by symmetry;apply D6_RsampleW.
+    split; first by move=> x; rewrite Dinter.supp_def; exact/Hbound.
+    split; first by move=> x Hx; cut:= Hbij x _.
+    by move=> x; rewrite Dinter.supp_def => Hx; cut:= Hbij x _.
+  by symmetry; apply/D6_RsampleW.
 qed.
 
 lemma prD6 : forall k &m, Pr[D6.sample() @ &m : res = k] = 
       if 1 <= k && k <= 4 then 1%r/4%r else 0%r.
 proof.
-  intros k &m. 
+  move=> k &m. 
   rewrite -(_:Pr[D4.sample() @ &m : res = k] = Pr[D6.sample() @ &m : res = k]).
     by byequiv (D4_D6 (fun x, x) (fun x, x) _ _).
   by apply (prD4 k &m).
